x86/AsmBuiltinInline.v
@@ -1,0 +1,468 @@
+(* ******************** *)
+(* Author: Xiangzhe Xu  *)
+(*         Zhenguo Yin  *)
+(* Date:   Aug 12, 2020 *)
+(* ******************** *)
+Require Import Coqlib Integers AST Memdata Maps.
+Require Import Events.
+Require Import Asm Asmgen.
+Require Import Errors.
+Require Import Memtype.
+Require Import Globalenvs.
+Require Import String.
+Require Import AsmLabelNew.
+Require Import Conventions1.
+Import ListNotations.
+
+Local Open Scope error_monad_scope.
+
+Section FUNCTION_SG.
+
+Variables (cur_func: function).
+  
+Definition option_ffpu := true.
+
+Definition _Plea r addr :=
+  if Archi.ptr64 then Pleaq r addr else Pleal r addr.
+
+Definition linear_addr reg ofs := 
+  Addrmode (Some reg) None (inl ofs).
+
+Definition global_addr id ofs := 
+  Addrmode None None (inr(id, ofs)).
+
+Definition addressing_of_builtin_arg arg := 
+  match arg with
+  | BA (IR r) => OK (linear_addr r 0)
+  | BA_addrstack ofs => OK (linear_addr RSP (Ptrofs.unsigned ofs))
+  | BA_addrglobal id ofs => OK (global_addr id ofs)
+  | _ => Error (msg "addressing_of_builtin_arg: builtin argument not supported")
+  end.
+
+Definition offset_addressing a delta :=
+  let '(Addrmode base ofs cst) := a in
+  let disp :=            
+      match cst with
+      | inl n => inl (n + delta)
+      | inr (id, n) => inr (id, Ptrofs.add n (Ptrofs.repr delta))
+      end in
+  Addrmode base ofs disp.
+
+(* Handling of memcpy *)
+
+(* Unaligned memory accesses are quite fast on IA32, so use large
+   memory accesses regardless of alignment. *)
+
+Fixpoint copy (fuel:nat) (src dst:addrmode) (sz:Z) : res (list instruction) :=
+  match fuel with
+  | O => OK []
+  | S fuel' =>
+    if zle 8 sz && Archi.ptr64 then 
+      do instrs <- copy fuel' (offset_addressing src 8) (offset_addressing dst 8) (sz - 8);
+      OK ([Pmovq_rm RCX src; Pmovq_mr dst RCX] ++ instrs)
+    else if zle 8 sz && option_ffpu then 
+      do instrs <- copy fuel' (offset_addressing src 8) (offset_addressing dst 8) (sz - 8);
+      OK ([Pmovsq_rm XMM7 src; Pmovsq_mr dst XMM7] ++ instrs)
+    else if zle 4 sz then 
+      do instrs <- copy fuel' (offset_addressing src 4) (offset_addressing dst 4) (sz - 4);
+      OK ([Pmovl_rm RCX src; Pmovl_mr dst RCX] ++ instrs)
+    else if zle 2 sz then
+      do instrs <- copy fuel' (offset_addressing src 2) (offset_addressing dst 2) (sz - 2);
+      OK ([Pmovw_rm RCX src; Pmovw_mr dst RCX] ++ instrs)
+    else if zle 1 sz then
+      do instrs <- copy fuel' (offset_addressing src 1) (offset_addressing dst 1) (sz - 1);
+      OK ([Pmovb_rm RCX src; Pmovb_mr dst RCX] ++ instrs)
+    else 
+      OK []
+  end.
+
+Definition expand_builtin_memcpy_small (sz al:Z) (src dst: builtin_arg preg) : res (list instruction) :=
+  do asrc <- (addressing_of_builtin_arg src);
+  do adst <- (addressing_of_builtin_arg dst);
+  copy (Z.to_nat sz) asrc adst sz.
+
+Definition crbit_arg_dec (c1 c2: crbit) : {c1 = c2} + {c1 <> c2}.
+  decide equality.
+Qed.
+
+Definition builtin_arg_dec (a1 a2: builtin_arg preg) : {a1 = a2} + {a1 <> a2}.
+  decide equality; try decide equality; try apply Ptrofs.eq_dec.
+  - apply ireg_eq.
+  - apply freg_eq.
+  - apply crbit_arg_dec.
+  - apply Int.eq_dec.
+  - apply Int64.eq_dec.
+  - apply Floats.Float.eq_dec.
+  - apply Floats.Float32.eq_dec.
+Qed.
+
+Definition expand_builtin_memcpy_big (sz al:Z) (src dst: builtin_arg preg) : res (list instruction) :=
+  do sinstrs <-
+      if builtin_arg_dec src (BA (IR RSI)) 
+      then OK []
+      else (do a <- addressing_of_builtin_arg src;
+              OK [_Plea RSI a]);
+  do dinstrs <-
+      if builtin_arg_dec dst (BA (IR RDI))
+      then OK []
+      else (do a <- addressing_of_builtin_arg dst;
+              OK [_Plea RDI a]);
+  let i1 := Pmovl_ri RCX (Int.repr (sz / 4)) in
+  let i2 := Prep_movsl in
+  let is1 := if zle 2 (sz mod 4) then [Pmovsw] else [] in
+  let is2 := if zle 1 (sz mod 2) then [Pmovsb] else [] in
+  OK (sinstrs ++ dinstrs ++ [i1; i2] ++ is1 ++ is2).
+  
+Definition expand_builtin_memcpy (sz al:Z) (args: list (builtin_arg preg)) : res (list instruction) :=
+  do r <-
+     match args with 
+     | [d; s] => OK (d, s) 
+     | _ => Error (msg "Error in expanding builtin memcpy: Wrong number of arguments")
+     end;
+  let '(dst, src) := r in
+  if zle sz 32 
+  then expand_builtin_memcpy_small sz al src dst
+  else expand_builtin_memcpy_big sz al src dst.
+
+Definition expand_builtin_vload_common chunk addr res :=
+  match chunk, res with
+  | Mint8unsigned, BR(IR res) =>
+     OK [Pmovzb_rm res addr]
+  | Mint8signed, BR(IR res) =>
+     OK [Pmovsb_rm res addr]
+  | Mint16unsigned, BR(IR res) =>
+     OK [Pmovzw_rm res addr]
+  | Mint16signed, BR(IR res) =>
+     OK [Pmovsw_rm res addr]
+  | Mint32, BR(IR res) =>
+     OK [Pmovl_rm res addr]
+  | Mint64, BR(IR res) =>
+     OK [Pmovq_rm res addr]
+  | Mint64, BR_splitlong (BR(IR res1)) (BR(IR res2)) =>
+     let addr' := offset_addressing addr 4 in
+     if negb (Asmgen.addressing_mentions addr res2) then
+       OK [Pmovl_rm res2 addr; Pmovl_rm res1 addr']
+     else
+       OK [Pmovl_rm res1 addr'; Pmovl_rm res2 addr] 
+  | Mfloat32, BR(FR res) =>
+     OK [Pmovss_fm res addr]
+  | Mfloat64, BR(FR res) =>
+     OK [Pmovsd_fm res addr]
+  | _, _ =>
+    Error [MSG "Error in expand_builtin_vload_common"]
+  end.
+
+Definition expand_builtin_vload chunk args res :=
+  match args with
+  | [addr] =>
+    do addr' <- addressing_of_builtin_arg addr;
+    expand_builtin_vload_common chunk addr' res
+  | _ => Error [MSG "Error in expand_builtin_vload"]
+  end.
+
+Definition expand_builtin_vstore_common chunk addr src tmp:=
+  match chunk, src with
+  | (Mint8signed | Mint8unsigned), BA(IR src) =>
+    if Archi.ptr64 || Asmgen.low_ireg src then
+      OK [Pmovb_mr addr src]
+    else
+      OK [Pmov_rr tmp src; Pmovb_mr addr tmp]
+  | (Mint16signed | Mint16unsigned), BA(IR src) =>
+    OK [Pmovw_mr addr src]
+  | Mint32, BA(IR src) =>
+    OK [Pmovl_mr addr src]
+  | Mint64, BA(IR src) =>
+    OK [Pmovq_mr addr src]
+  | Mint64, BA_splitlong (BA(IR src1)) (BA(IR src2)) =>
+    let addr' := offset_addressing addr 4 in
+    OK [Pmovl_mr addr src2; Pmovl_mr addr' src1]
+  | Mfloat32, BA(FR src) =>
+    OK [Pmovss_mf addr src]
+  | Mfloat64, BA(FR src) =>
+    OK [Pmovsd_mf addr src]
+  | _, _ =>
+    Error [MSG "Error in expand_builtin_vstore_common"]
+  end.
+
+Definition expand_builtin_vstore chunk args :=
+  match args with
+  | [addr; src] =>
+    do addr' <- addressing_of_builtin_arg addr;
+    let tmp := if Asmgen.addressing_mentions addr' RAX
+               then RCX
+               else RAX in
+     expand_builtin_vstore_common chunk addr' src tmp
+  | _ => Error [MSG "Error in expand_builtin_vstore"]
+  end.
+
+Definition expand_fma args result i132 i213 i231 :=
+  match args, result with
+  | [BA(FR a1); BA(FR a2); BA(FR a3)], BR(FR result) =>
+    if freg_eq result a1 then
+      OK [i132 a1 a3 a2] (* a1 * a2 + a3 *) else
+      if freg_eq result a2 then
+        OK [i213 a2 a1 a3] (* a1 * a2 + a3 *) else
+        if freg_eq result a3 then
+          OK [i231 a3 a1 a2] (* a1 * a2 + a3 *) else
+          (* a1 * a2 + res *)
+          OK [Pmovsd_ff result a3; i231 result a1 a2]
+  | _, _ => Error [MSG "ill-formed fma builtin"]
+  end.
+
+(* Copy from ccelf-no-perm x86/Conventions1.v *)
+(** [size_arguments s] returns the number of [Outgoing] slots used
+  to call a function with signature [s]. *)
+Require Import Machregs.
+Definition int_param_regs := DI :: SI :: DX :: CX :: R8 :: R9 :: nil.
+Definition float_param_regs := X0 :: X1 :: X2 :: X3 :: X4 :: X5 :: X6 :: X7 :: nil.
+
+Fixpoint size_arguments_32
+    (tyl: list typ) (ofs: Z) {struct tyl} : Z :=
+  match tyl with
+  | nil => ofs
+  | ty :: tys => size_arguments_32 tys (ofs + typesize ty)
+  end.
+
+Fixpoint size_arguments_64 (tyl: list typ) (ir fr ofs: Z) {struct tyl} : Z :=
+  match tyl with
+  | nil => ofs
+  | (Tint | Tlong | Tany32 | Tany64) :: tys =>
+      match list_nth_z int_param_regs ir with
+      | None => size_arguments_64 tys ir fr (ofs + 2)
+      | Some ireg => size_arguments_64 tys (ir + 1) fr ofs
+      end
+  | (Tfloat | Tsingle) :: tys =>
+      match list_nth_z float_param_regs fr with
+      | None => size_arguments_64 tys ir fr (ofs + 2)
+      | Some freg => size_arguments_64 tys ir (fr + 1) ofs
+      end
+  end.
+
+Definition size_arguments (s: signature) : Z :=
+  if Archi.ptr64
+  then size_arguments_64 s.(sig_args) 0 0 0
+  else size_arguments_32 s.(sig_args) 0.
+
+(* End Copy *)
+
+Definition expand_builtin_va_start_32 r :=
+  if cc_vararg (sig_cc (fn_sig cur_func)) then
+    (* fn_stacksize correct? *)
+    let sz := align (fn_stacksize cur_func) 8 - size_chunk Mptr in
+    let t0 := Z.add sz 4 in
+    (* let t0 := Z.add (fn_stacksize cur_func) 4 in *)
+    let t1 := Z.mul 4 (size_arguments (fn_sig cur_func)) in
+    let ofs := Z.add t0 t1 in
+    OK [Pleal RAX (linear_addr RSP ofs);
+       Pmovl_mr (linear_addr r 0) RAX]
+  else
+    Error [MSG "Fatal error: va_start used in non-vararg function"].
+         
+(* Expand builtin inline assembly *)
+Definition expand_builtin_inline name args res :=
+  match name,args,res with
+  (* Integer arithmetic *)
+  | ("__builtin_bswap"%string | "__builtin_bswap32"%string), [BA(IR a1)], BR(IR a2) =>
+    let i:= if negb (ireg_eq a1 a2) then
+              [Pmov_rr a2 a1] else
+              [] in
+    OK (i++[Pbswap32 a2])
+  | "__builtin_bswap64"%string, [BA(IR a1)], BR(IR a2) =>
+    let i:= if negb (ireg_eq a1 a2) then
+              [Pmov_rr a2 a1] else
+              [] in
+    OK (i++[Pbswap64 a2])
+  | "__builtin_bswap64"%string, [BA_splitlong (BA(IR ah)) (BA(IR al))],
+    BR_splitlong (BR(IR rh)) (BR(IR rl)) =>
+    if (ireg_eq ah RAX && ireg_eq al RDX && ireg_eq rh RDX &&
+        ireg_eq rl RAX) then
+      OK [Pbswap32 RAX; Pbswap32 RDX]
+    else
+      Error (msg "Error in expanding of builtin: __builtin_bswap64 arguments incorrect")
+  | "__builtin_bswap16"%string, [BA(IR a1)], BR(IR a2) =>
+    let i:= if negb (ireg_eq a1 a2) then
+              [Pmov_rr a2 a1] else
+              [] in
+    OK (i++[Pbswap16 a2])
+  | ("__builtin_clz"%string|"__builtin_clzl"%string), [BA(IR a1)], BR(IR a2) =>
+     OK [Pbsrl a2 a1; Pxorl_ri a2 (Int.repr 31)]
+  | "__builtin_clzll"%string, [BA(IR a1)], BR(IR a2) =>
+    OK [Pbsrq a2 a1; Pxorl_ri a2 (Int.repr 63)]
+  | "__builtin_clzll"%string, [BA_splitlong (BA (IR ah)) (BA (IR al))], BR(IR ar) =>
+    let lbl1 := new_label tt in
+    let lbl2 := new_label tt in
+    OK [Ptestl_rr ah ah; Pjcc Cond_e lbl1; Pbsrl ar ah; Pxorl_ri ar (Int.repr 31);
+       Pjmp_l lbl2; Plabel lbl1; Pbsrl ar al; Pxorl_ri ar (Int.repr 63); Plabel lbl2]
+  | ("__builtin_ctz"%string | "__builtin_ctzl"%string), [BA(IR a1)], BR(IR a2) =>
+    OK [Pbsfl a2 a1]
+  | "__builtin_ctzll"%string, [BA(IR a1)], BR(IR a2) =>
+    OK [Pbsfq a2 a1]
+  | "__builtin_ctzll"%string, [BA_splitlong (BA (IR ah)) (BA (IR al))], BR(IR ar) =>
+    let lbl1 := new_label tt in
+    let lbl2 := new_label tt in
+    OK [Ptestl_rr al al; Pjcc Cond_e lbl1; Pbsfl ar al; Pjmp_l lbl2; Plabel lbl1;
+       Pbsfl ar ah; Paddl_ri ar (Int.repr 32); Plabel lbl2]
+  (* Float arithmetic *)
+  | "__builtin_fabs"%string, [BA(FR a1)], BR(FR ar) =>
+    let i:= if negb (freg_eq a1 ar) then
+              [Pmovsd_ff ar a1] else
+              [] in
+    OK (i++[Pabsd ar])
+  (* This ensuar that need_masks is set to true *)
+  | "__builtin_fsqrt"%string, [BA(FR a1)], BR(FR ar) =>
+    OK [Psqrtsd ar a1]
+  | "__builtin_fmax"%string, [BA(FR a1); BA(FR a2)], BR(FR ar) =>
+    let i := [Pmovsd_ff ar a1; Pmaxsd ar a2] in
+    if freg_eq ar a1 then
+      OK ([Pmaxsd ar a2]++i) else
+      if freg_eq ar a2 then
+        OK ([Pmaxsd ar a1]++i) else
+	OK i
+  | "__builtin_fmin"%string, [BA(FR a1); BA(FR a2)], BR(FR ar) =>
+    let i := [Pmovsd_ff ar a1; Pminsd ar a2] in
+    if freg_eq ar a1 then
+      OK ([Pminsd ar a2]++i) else
+      if freg_eq ar a2 then
+        OK ([Pminsd ar a1]++i) else
+	OK i
+  | "__builtin_fmadd"%string,  _, _ =>
+      expand_fma args res
+        (fun r1 r2 r3 => Pfmadd132 r1 r2 r3)
+        (fun r1 r2 r3 => Pfmadd213 r1 r2 r3)
+        (fun r1 r2 r3 => Pfmadd231 r1 r2 r3)
+  | "__builtin_fmsub"%string,  _, _ =>
+      expand_fma args res
+        (fun r1 r2 r3 => Pfmsub132 r1 r2 r3)
+        (fun r1 r2 r3 => Pfmsub213 r1 r2 r3)
+        (fun r1 r2 r3 => Pfmsub231 r1 r2 r3)
+  | "__builtin_fnmadd"%string,  _, _ =>
+      expand_fma args res
+        (fun r1 r2 r3 => Pfnmadd132 r1 r2 r3)
+        (fun r1 r2 r3 => Pfnmadd213 r1 r2 r3)
+        (fun r1 r2 r3 => Pfnmadd231 r1 r2 r3)
+  | "__builtin_fnmsub"%string,  _, _ =>
+      expand_fma args res
+        (fun r1 r2 r3 => Pfnmsub132 r1 r2 r3)
+        (fun r1 r2 r3 => Pfnmsub213 r1 r2 r3)
+        (fun r1 r2 r3 => Pfnmsub231 r1 r2 r3)
+  (* 64-bit integer arithmetic *)
+  | "__builtin_negl"%string, [BA_splitlong (BA(IR ah)) (BA(IR al))],
+    BR_splitlong (BR(IR rh)) (BR(IR rl)) =>
+    if (ireg_eq ah RDX && ireg_eq al RAX && ireg_eq rh RDX &&
+        ireg_eq rl RAX) then
+      OK [Pnegl RAX; Padcl_ri RDX Int.zero; Pnegl RDX]
+    else
+      Error (msg "Error in expanding of builtin: __builtin_negl arguments incorrect")  
+  | "__builtin_addl"%string, [BA_splitlong (BA(IR ah)) (BA(IR al));
+                              BA_splitlong (BA(IR bh)) (BA(IR bl))],
+    BR_splitlong (BR(IR rh)) (BR(IR rl)) =>
+    if (ireg_eq ah RDX && ireg_eq al RAX && ireg_eq bh RCX &&
+        ireg_eq bl RBX && ireg_eq rh RDX && ireg_eq rl RAX) then
+      OK [Paddl_rr RAX RBX; Padcl_rr RDX RCX]
+    else
+      Error (msg "Error in expanding of builtin: __builtin_addl arguments incorrect")             
+  | "__builtin_subl"%string, [BA_splitlong (BA(IR ah)) (BA(IR al));
+                              BA_splitlong (BA(IR bh)) (BA(IR bl))],
+    BR_splitlong (BR(IR rh)) (BR(IR rl)) =>
+    if (ireg_eq ah RDX && ireg_eq al RAX && ireg_eq bh RCX &&
+        ireg_eq bl RBX && ireg_eq rh RDX && ireg_eq rl RAX) then
+      OK [Psubl_rr RAX RBX; Psbbl_rr RDX RCX]
+    else
+      Error (msg "Error in expanding of builtin: __builtin_subl arguments incorrect")
+  | "__builtin_mull"%string, [BA(IR a); BA(IR b)],
+    BR_splitlong (BR(IR rh)) (BR(IR rl)) =>
+    if (ireg_eq a RAX && ireg_eq b RDX && ireg_eq rh RDX &&
+        ireg_eq rl RAX) then
+      OK [Pmull_r RDX]
+    else
+      Error (msg "Error in expanding of builtin: __builtin_mull arguments incorrect")
+  (* Memory accesses *)
+  | "__builtin_read16_reversed"%string, [BA(IR a1)], BR(IR ar) =>
+     OK [Pmovzw_rm ar (linear_addr a1 0); Pbswap16 ar]
+  | "__builtin_read32_reversed"%string, [BA(IR a1)], BR(IR ar)  =>
+     OK [Pmovl_rm ar (linear_addr a1 0); Pbswap32 ar]
+  | "__builtin_write16_reversed"%string, [BA(IR a1); BA(IR a2)], _  =>
+    let tmp := if ireg_eq a1 RCX then RDX else RCX in
+    let i := if negb (ireg_eq a2 tmp) then
+               [Pmov_rr tmp a2] else
+               [] in
+    OK (i++[Pbswap16 tmp; Pmovw_mr (linear_addr a1 0) tmp])
+  | "__builtin_write32_reversed"%string, [BA(IR a1); BA(IR a2)], _  =>
+    let tmp := if ireg_eq a1 RCX then RDX else RCX in
+    let i := if negb (ireg_eq a2 tmp) then
+               [Pmov_rr tmp a2] else
+               [] in
+    OK (i++[Pbswap32 tmp; Pmovl_mr (linear_addr a1 0) tmp])
+  (* Vararg stuff *)
+  | "__builtin_va_start"%string, [BA(IR a)], _ =>
+    if (ireg_eq a RDX) then
+      if Archi.ptr64
+      then Error (msg "Error vaarg in x86_64")
+      else expand_builtin_va_start_32 a       
+    else
+      Error (msg "Error in expanding of builtin: __builtin_va_start arguments incorrect")
+  (* Synchronization *)
+  | "__builtin_membar"%string, [], _ =>
+    OK []
+  (* no operation *)
+  | "__builtin_nop"%string, [], _  =>
+    OK [Pmov_rr RAX RAX]
+  | _ ,_ ,_  =>  Error [MSG "Error in expanding of builtin: " ; MSG name]
+  end.
+
+Definition transf_instr (i: instruction): res (list instruction) :=
+  match i with
+  | Pbuiltin ef args res =>
+    match ef with
+    | EF_memcpy sz al =>
+      expand_builtin_memcpy sz al args
+    | EF_builtin name sg =>
+      do i <- expand_builtin_inline name args res;
+      OK i
+    | EF_vload chunk =>
+      expand_builtin_vload chunk args res
+    | EF_vstore chunk =>
+      expand_builtin_vstore chunk args
+    | EF_annot (* SANCC *) _ text targs =>
+      OK [Pnop]
+    | EF_annot_val (* SANCC *) _ text targ =>
+      OK [Pnop]
+    | EF_inline_asm text sg clob =>
+      Error [MSG "Unsupported Builtin Elimination: inline_asm"]
+    | EF_debug kind text targs =>
+      Error [MSG "Unsupported Builtin Elimination: debug"]
+    | _ => Error [MSG "Unsupported Builtin Elimination: unknown"]
+    end
+  | _ => OK [i]
+  end.
+
+Definition acc_transl_instr (r:res code) (i:instruction) :=
+  do acc_i <- r;
+  do i' <- transf_instr i;
+  OK (acc_i ++ i').
+  
+Definition transl_code (c:code) : res code :=
+  do code <- fold_left acc_transl_instr c (OK []);
+  OK (code).
+
+End FUNCTION_SG.
+
+Definition transf_function (f: function) : res function :=
+  (* make sure that code can not have relative jumps*)
+  if func_no_jmp_rel_dec f then
+    do tt <-  set_current_function f;
+    do fn_code' <- transl_code f (fn_code f);
+    OK {|
+        fn_sig := fn_sig f;
+        fn_code := fn_code';
+        fn_stacksize := fn_stacksize f;
+        fn_ofs_link := fn_ofs_link f (* SANCC *)
+      |}
+  else
+    Error [MSG "Code contains relative jumps"].
+
+Definition transf_fundef (f: Asm.fundef) : res Asm.fundef :=
+  transf_partial_fundef transf_function f.
+
+Definition transf_program (p: Asm.program) : res Asm.program :=
+  transform_partial_program transf_fundef p.
