x86/AsmLabelNew.v
@@ -1,0 +1,13 @@
+(* ******************** *)
+(* Author: Zhenguo Yin  *)
+(* Date:   Aug 30, 2020 *)
+(* ******************** *)
+
+Require Import Coqlib Integers AST Maps.
+Require Import Asm.
+Require Import Errors.
+
+(** Set Current Function *)
+Parameter set_current_function : function -> res unit.
+(** Generate New Lable *)
+Parameter new_label : unit -> label.
