x86/AsmPseudoInstr.v
@@ -1,0 +1,76 @@
+(* ******************** *)
+(* Author: Xiangzhe Xu  *)
+(*         Zhenguo Yin  *)
+(* Date:   Aug 12, 2020 *)
+(* ******************** *)
+Require Import Coqlib Integers AST Maps.
+Require Import Events.
+Require Import Asm.
+Require Import Errors.
+Require Import Memtype.
+Require Import Globalenvs.
+Require Import AsmLabelNew.
+Import ListNotations.
+
+Local Open Scope error_monad_scope.
+
+Definition neg_cond (cond:testcond) :=
+  match cond with
+  | Cond_e => Cond_ne
+  | Cond_ne => Cond_e
+  | Cond_b => Cond_ae
+  | Cond_be => Cond_a
+  | Cond_ae => Cond_b
+  | Cond_a => Cond_be
+  | Cond_l => Cond_ge
+  | Cond_le => Cond_g
+  | Cond_ge => Cond_l
+  | Cond_g => Cond_le
+  | Cond_p => Cond_np
+  | Cond_np => Cond_p
+  end.
+
+Definition transf_instr (i: instruction) (code: code) : res (list instruction) :=
+  match i with
+  | Psetcc c rd =>
+   OK [Psetcc c rd; Pmovzb_rr rd rd]
+  | Pjcc2 cond1 cond2 lbl =>
+    let lbl' := new_label tt in
+    let i1 := Pjcc (neg_cond cond1) lbl' in
+    let i2 := Pjcc cond2 lbl in
+    let i3 := Plabel lbl' in
+    OK ([i1]++[i2]++[i3])
+  (* SANCC  *)
+  (* | Pbswap16 rd => *)
+  (*   OK [Prolw_ri rd (Int.repr 8)] *)
+  |_ => OK [i] 
+  end.
+
+Definition acc_transl_instr (c: code) (r:res code) (i:instruction) :=
+  do acc_i <- r;
+  do i' <- transf_instr i c;
+  OK (acc_i ++ i').
+  
+Definition transl_code (c: code) : res code :=
+  do code <- fold_left (acc_transl_instr c) c (OK []);
+  OK (code).
+
+Definition transf_function (f: function) : res function :=
+  (* make sure that code can not have relative jumps*)
+  if func_no_jmp_rel_dec f then
+    do tt <-  set_current_function f;
+    do fn_code' <- transl_code (fn_code f);
+    OK {|
+        fn_sig := fn_sig f;
+        fn_code := fn_code';
+        fn_stacksize := fn_stacksize f;
+        fn_ofs_link := fn_ofs_link f
+      |}
+  else
+    Error [MSG "Code contains relative jumps"].
+
+Definition transf_fundef (f: Asm.fundef) : res Asm.fundef :=
+  transf_partial_fundef transf_function f.
+
+Definition transf_program (p: Asm.program) : res Asm.program :=
+  transform_partial_program transf_fundef p.
