x86/AsmStructRet.v
@@ -1,0 +1,64 @@
+(* ******************** *)
+(* Author: Zhenguo Yin  *)
+(* Date:   Aug 28, 2020 *)
+(* ******************** *)
+Require Import Coqlib Integers AST Maps.
+Require Import Events.
+Require Import Asm.
+Require Import Errors.
+Require Import Memtype.
+Require Import Globalenvs.
+Import ListNotations.
+
+Local Open Scope error_monad_scope.
+
+Definition transf_instr (i: instruction) (cur_sg: signature) : res (list instruction) :=
+  match i with
+  | Pcall_r _ sg =>
+    if (negb Archi.ptr64) && cc_structret (sig_cc sg) then
+      let i1 := Psubl_ri RSP (Int.repr 4) in
+      let i2 := Pmovl_mr (Addrmode (Some RSP) None (inl 0)) RAX in
+      OK ([i]++[i1]++[i2]) else
+      OK [i]
+  | Pcall_s _ sg =>
+    if (negb Archi.ptr64) && cc_structret (sig_cc sg) then
+      let i1 := Psubl_ri RSP (Int.repr 4) in
+      let i2 := Pmovl_mr (Addrmode (Some RSP) None (inl 0)) RAX in
+      OK ([i]++[i1]++[i2]) else
+      OK [i]
+  | Pret =>
+    if (negb Archi.ptr64) && cc_structret (sig_cc cur_sg) then
+      let i1 := Pmovl_rm RAX (Addrmode (Some RSP) None (inl 0)) in
+      let i2 := Pret_iw (Int.repr 4) in
+      OK ([i1]++[i2]) else
+      OK [i]
+  |_ => OK [i] 
+  end.
+
+Definition acc_transl_instr (sg: signature) (r:res code) (i:instruction) :=
+  do acc_i <- r;
+  do i' <- transf_instr i sg;
+  OK (acc_i ++ i').
+  
+Definition transl_code (c: code) (sg: signature) : res code :=
+  do code <- fold_left (acc_transl_instr sg) c (OK []);
+  OK (code).
+
+Definition transf_function (f: function) : res function :=
+  (* make sure that code can not have relative jumps*)
+  if func_no_jmp_rel_dec f then
+    do fn_code' <- transl_code (fn_code f) (fn_sig f);
+    OK {|
+        fn_sig := fn_sig f;
+        fn_code := fn_code';
+        fn_stacksize := fn_stacksize f;
+        fn_ofs_link := fn_ofs_link f
+      |}
+  else
+    Error [MSG "Code contains relative jumps"].
+
+Definition transf_fundef (f: Asm.fundef) : res Asm.fundef :=
+  transf_partial_fundef transf_function f.
+
+Definition transf_program (p: Asm.program) : res Asm.program :=
+  transform_partial_program transf_fundef p.
