x86/Asmlabelgen.v
@@ -1,0 +1,105 @@
+(* *******************  *)
+(* Author: Xiangzhe Xu  *)
+(* Date:   Sep 16, 2019 *)
+(* *******************  *)
+
+
+
+
+Require Import Coqlib Integers AST Maps.
+Require Import Events.
+Require Import Asm.
+Require Import Errors.
+Require Import Memtype.
+Require Import Globalenvs .
+Import ListNotations.
+
+Local Open Scope error_monad_scope.
+
+Section INSTRSIZE.
+
+  Variable instr_size : instruction -> Z. (* SANCC *)
+
+Fixpoint findAllLabel (l: list label)(all:list instruction): res (list Z) :=
+  match l with
+  |[] => OK []
+  |h :: t =>
+   match label_pos instr_size h 0 all (*SANCC*)with
+   |None => Error (msg"Label not found")
+   |Some pos =>
+    do tail <-  (findAllLabel t all);
+      OK (pos::tail)
+   end
+  end.
+
+Definition transl_instr (i: instruction) (ofs:Z) (code:code) : res instruction :=
+  let sz := instr_size i in
+  match i with
+  |Pjmp_l lbl =>
+   match label_pos instr_size lbl 0 code with
+   (* label not found *)
+   |None =>   Error (msg"Label not found")
+   |Some pos =>
+    let relOfs :=  pos - (ofs+sz)  in
+    OK (Pjmp_l_rel relOfs)
+   end
+
+  |Pjcc cond lbl =>
+   match label_pos instr_size lbl 0 code with
+   (* label not found *)
+   |None =>  Error (msg"Label not found")
+   |Some pos =>
+    let relOfs := pos - (ofs+sz) in
+    OK (Pjcc_rel cond relOfs)
+   end
+
+  |Pjcc2 cond1 cond2 lbl =>
+   match label_pos instr_size lbl 0 code with
+   (* label not found *)
+   |None =>  Error (msg"Label not found")
+   |Some pos =>
+    let relOfs := pos - (ofs+sz) in
+    OK (Pjcc2_rel cond1 cond2 relOfs)
+   end
+
+  (* Do this after symbol table generation*)
+  |Pjmptbl r tbl =>
+   do lst <-  findAllLabel tbl code;
+   let ofsLst := map (Zplus (-( sz + ofs))) lst in
+   OK (Pjmptbl_rel r ofsLst)
+          
+  |_ =>
+   OK i 
+  end.
+
+
+Definition acc_transl_instr c r i :=
+  do r' <- r;
+    let '(ofs, code) := r' in
+    do i' <- transl_instr i ofs c;
+      OK (ofs + instr_size i, (i' :: code)).
+  
+Definition transl_code (c:code) : res code :=
+  do rs <- 
+     fold_left (acc_transl_instr c)
+               c
+               (OK (0, []));
+  let '(_, c') := rs in
+  OK (rev c').
+
+
+Definition trans_function (f: function) :res function :=
+  if func_no_jmp_rel_dec f then 
+    do instrs <- transl_code (fn_code f);
+      OK (mkfunction (fn_sig f) instrs (fn_stacksize f) (fn_ofs_link f))
+  else
+    Error (msg "Some source function contains relative jumps").
+
+Definition transf_fundef (f: Asm.fundef) : res Asm.fundef :=
+  transf_partial_fundef trans_function f.
+
+Definition transf_program (p: Asm.program) : res Asm.program :=
+  transform_partial_program transf_fundef p.
+
+End INSTRSIZE.
+
