Makefile
@@ -114,7 +114,13 @@ BACKEND=\
   Asm.v Asmgen.v Asmgenproof0.v Asmgenproof1.v \
   AsmRegs.v AsmFacts.v Asmgenproof.v \
   SSAsm.v SSAsmproof.v \
-  RealAsm.v RealAsmgen.v RealAsmproof.v PseudoInstructions.v PseudoInstructionsproof.v
+  RealAsm.v RealAsmgen.v RealAsmproof.v PseudoInstructions.v PseudoInstructionsproof.v \
+  AsmLabelNew.v AsmBuiltinInline.v \
+  AsmStructRet.v \
+  AsmFloatLiteral.v SymbolString.v\
+  AsmPseudoInstr.v \
+  Asmlabelgen.v \
+  
 # C front-end modules (in cfrontend/)
 
 CFRONTEND=Ctypes.v Cop.v Csyntax.v Csem.v Ctyping.v Cstrategy.v Cexec.v \
